MicroPolicies/Merged.v
@@ -1,0 +1,106 @@
+Require Import Common.Definitions.
+
+From CoqUtils Require Import hseq word.
+From extructures Require Import fmap.
+From mathcomp Require Import ssreflect ssrfun ssrbool eqtype ssrnat seq.
+
+Require Import Types.
+Require Import Transitional.
+Require Import MicroPolicies.Utils MicroPolicies.LRC MicroPolicies.Symbolic Intermediate.Machine.
+Require Import CompCert.Events.
+
+Set Implicit Arguments.
+Unset Strict Implicit.
+Unset Printing Implicit Defensive.
+Import DoNotation.
+
+Variant instr :=
+| MrNop : instr
+| MrLabel : plabel -> instr
+| MrConst : imvalue -> register -> instr
+| MrMov : register  -> register -> instr
+| MrBinop : binop -> register -> register -> register -> instr
+| MrLoad : register -> register -> instr
+| MrStore : register -> register -> instr
+| MrJump : register -> instr
+| MrBnz : register -> plabel -> instr
+| MrJal : imvalue -> instr
+| MrHalt : instr.
+
+Context {mt : machine_types}
+  {ops : machine_ops mt}.
+
+
+(* Memory model and definition are the same as defined in LRC.v *)
+(* TODO : this must be rewritten explicitely as sym_lrc contains transfer *)
+(*
+Notation state := (@Symbolic.state mt sym_lrc).
+Notation State := (@Symbolic.State mt sym_lrc).
+ *)
+
+Local Notation word := (mword mt).
+Let atom := (atom word).
+
+Local Notation memory := {fmap word -> atom (Symbolic.tag_type lrc_tags Symbolic.M)}.
+Local Notation registers := {fmap register -> atom (Symbolic.tag_type lrc_tags Symbolic.R)}.
+
+Record state := State {
+  mem : memory;
+  regs : registers;
+  pc : atom (Symbolic.tag_type lrc_tags Symbolic.P)
+}.
+
+Notation instr_rules := LRC.instr_rules.
+Notation state_ev := (state * option event)%type.
+
+Notation update := (@Symbolic.update mt).
+(*
+Inductive update :=
+  | RegWrite : register -> word -> update
+  | RegRead  : register -> update
+  | MemWrite : word -> word -> update
+  | MemRead : word -> update
+.*)
+
+(*
+Definition vovec (op : opcode) : Type := Symbolic.ovec lrc_tags op.
+Notation vovec_ev op := ((vovec op) * option event)%type.
+
+Record ivec : Type := IVec {
+  op  : opcode;
+  tpc : Symbolic.tag_type lrc_tags Symbolic.P;
+  ti  : Symbolic.instr_tag op;
+  ts  : hseq Symbolic.tag_type (vinputs op);
+  tni : option (Symbolic.tag_type Symbolic.M)
+}.*)
+
+
+Definition code := (seq (instr * mem_tag *  Component.id)).
+
+
+(* TODO: is this sufficiently expressive as a global environment? *)
+Definition global_env := NMap nat. (* label -> start of procedure (expressed as offset in code) *)
+
+
+Definition executing (cde : code) (pc : mword mt) (i : instr) (tg : mem_tag) (c : Component.id) : Prop :=
+  let off := Symbolic.convert (word.int_of_word pc) in
+  (off >= 0) % Z /\ nth_error cde (Z.to_nat off) = Some (i,tg,c).
+
+Definition next_state_updates (st : state) (op : opcode) (updts : seq update) : option state_ev :=
+  None. (*next_state_updates_and_pc st iv updts (vala (pc st)).+1.*)
+
+Inductive step (cde : code) (G : global_env) (st st' : state) (ev : option event) : Prop :=
+| step_nop : forall mem reg pc tpc i ti tg c
+               (ST   : st = State mem reg pc@tpc)
+               (PC   : mem pc = Some i@ti)
+               (INST : executing cde pc MrNop tg c), forall
+        (NEXT : next_state_updates st NOP [:: ] = Some (st', ev)),    step cde G st st' ev
+| step_nop' : forall pc tg c 
+               (INST : executing cde pc MrNop tg c)
+               (NO_EVENT : ev = None),
+    step cde G st st' ev.
+
+
+
+(* Definition eval_step (cde : code) (G : global_env) (st : state) : option (event * state) := *)
+
